Request-response functions with state on the server side

src/lib/communication/DY.Lib.Communication.Core.Invariants.fst
@@ -1,4 +1,4 @@
-module DY.Lib.Communication.API.Invariants
+module DY.Lib.Communication.Core.Invariants
 
 open Comparse
 open DY.Core
@@ -9,9 +9,8 @@ open DY.Lib.Crypto.AEAD.Split
 open DY.Lib.Event.Typed
 open DY.Lib.State.PrivateKeys
 open DY.Lib.State.Tagged
-open DY.Lib.State.Typed
 
-open DY.Lib.Communication.API
+open DY.Lib.Communication.Core
 
 #set-options "--fuel 0 --ifuel 0 --z3cliopt 'smt.qi.eager_threshold=100'"
 
@@ -33,38 +32,6 @@ val pkenc_crypto_predicates_communication_layer_and_tag:
   (string & pkenc_crypto_predicate)
 let pkenc_crypto_predicates_communication_layer_and_tag #cusages = 
   (comm_layer_pkenc_tag, pkenc_crypto_predicates_communication_layer)
-
-(*** AEAD Predicate ***)
-
-#push-options "--ifuel 1 --fuel 0"
-val aead_crypto_predicate_communication_layer: {|cusages:crypto_usages|} -> aead_crypto_predicate
-let aead_crypto_predicate_communication_layer #cusages = {
-  pred = (fun tr key_usage nonce msg ad ->
-    (match parse response_message msg with
-    | None -> False
-    | Some {id; payload} -> (
-      match parse authenticated_data ad with
-      | None -> False
-      | Some {client; server} -> (
-        event_triggered tr server (CommServerReceiveRequest server id payload) /\
-        (get_label tr id) `can_flow tr` (comm_label client server) /\
-        (get_label tr payload) `can_flow tr` (comm_label client server)
-      )
-    ))
-  );
-  pred_later = (fun tr1 tr2 key_usage nonce msg ad -> (
-    parse_wf_lemma response_message (bytes_well_formed tr1) msg;
-    parse_wf_lemma authenticated_data (bytes_well_formed tr1) ad;
-    ()
-  ))
-}
-#pop-options
-
-val aead_crypto_predicates_communication_layer_and_tag:
-  {|cusages:crypto_usages|} ->
-  (string & aead_crypto_predicate)
-let aead_crypto_predicates_communication_layer_and_tag #cusages =
-  (comm_layer_aead_tag, aead_crypto_predicate_communication_layer)
 
 (*** Sign Predicates ***)
 
@@ -104,54 +71,7 @@ val has_communication_layer_crypto_predicates:
   prop
 let has_communication_layer_crypto_predicates #cinvs =
   has_pkenc_predicate pkenc_crypto_predicates_communication_layer_and_tag /\
-  has_sign_predicate sign_crypto_predicates_communication_layer_and_tag /\
-  has_aead_predicate aead_crypto_predicates_communication_layer_and_tag
-
-
-(*** State Predicates ***)
-
-#push-options "--ifuel 2 --z3rlimit 25"
-let state_predicates_communication_layer {|crypto_invariants|}: local_state_predicate communication_states = {
-  pred = (fun tr prin sess_id st -> 
-    match st with
-    | ClientSendRequest {id; server; payload; key} -> (
-      let client = prin in
-      is_secret (comm_label client server) tr id /\
-      is_knowable_by (comm_label client server) tr payload /\
-      is_secret (comm_label client server) tr key
-    )
-    | ServerReceiveRequest {id; client; payload; key} -> (
-      let server = prin in
-      (exists client.
-        is_knowable_by (comm_label client server) tr id /\
-        is_knowable_by (comm_label client server) tr payload /\
-        is_knowable_by (comm_label client server) tr key
-      )
-    )
-    | ClientReceiveResponse {id; server; payload; key} -> (
-      let client = prin in
-      is_secret (comm_label client server) tr id /\
-      is_knowable_by (comm_label client server) tr payload /\
-      is_secret (comm_label client server) tr key
-    )
-  );
-  pred_later = (fun tr1 tr2 prin sess_id state -> ());
-  pred_knowable = (fun tr prin sess_id state -> ());
-}
-#pop-options
-
-val state_predicates_communication_layer_and_tag: 
-  {|crypto_invariants|} ->
-  dtuple2 string local_bytes_state_predicate
-let state_predicates_communication_layer_and_tag #cinvs =
-  (|local_state_communication_layer_session.tag, local_state_predicate_to_local_bytes_state_predicate (state_predicates_communication_layer #cinvs)|)
-
-val has_communication_layer_state_predicates:
-  {|protocol_invariants|} ->
-  prop
-let has_communication_layer_state_predicates #invs =
-  has_local_state_predicate state_predicates_communication_layer
- 
+  has_sign_predicate sign_crypto_predicates_communication_layer_and_tag
 
 (*** Event Predicates ***)
 
@@ -164,6 +84,7 @@ type comm_higher_layer_event_preds = {
     Lemma
     (requires
       send_conf tr1 sender receiver payload /\
+      bytes_well_formed tr1 payload /\
       tr1 <$ tr2
     )
     (ensures send_conf tr2 sender receiver payload)
@@ -175,6 +96,7 @@ type comm_higher_layer_event_preds = {
     Lemma
     (requires
       send_auth tr1 sender payload /\
+      bytes_well_formed tr1 payload /\
       tr1 <$ tr2
     )
     (ensures send_auth tr2 sender payload)
@@ -186,35 +108,10 @@ type comm_higher_layer_event_preds = {
     Lemma
     (requires
       send_conf_auth tr1 sender receiver payload /\
+      bytes_well_formed tr1 payload /\
       tr1 <$ tr2
     )
     (ensures send_conf_auth tr2 sender receiver payload)
-  ;
-  send_request: tr:trace -> client:principal -> server:principal -> payload:bytes -> prop;
-  send_request_later:
-    tr1:trace -> tr2:trace ->
-    client:principal -> server:principal -> payload:bytes ->
-    Lemma
-    (requires
-      send_request tr1 client server payload /\
-      tr1 <$ tr2
-    )
-    (ensures
-      send_request tr2 client server payload
-    )
-  ;
-  send_response: tr:trace -> server:principal -> payload:bytes -> prop;
-  send_response_later:
-    tr1:trace -> tr2:trace ->
-    server:principal -> payload:bytes ->
-    Lemma
-    (requires
-      send_response tr1 server payload /\
-      tr1 <$ tr2
-    )
-    (ensures
-      send_response tr2 server payload
-    )
 }
 
 val default_comm_higher_layer_event_preds: comm_higher_layer_event_preds
@@ -224,25 +121,19 @@ let default_comm_higher_layer_event_preds = {
   send_auth = (fun tr sender payload -> True);
   send_auth_later = (fun tr1 tr2 sender payload -> ());
   send_conf_auth = (fun tr sender receiver payload -> True);
-  send_conf_auth_later = (fun tr1 tr2 sender receiver payload -> ());
-  send_request = (fun tr client server payload -> True);
-  send_request_later = (fun tr1 tr2 client server payload -> ());
-  send_response = (fun tr server payload -> True);
-  send_response_later = (fun tr1 tr2 server payload -> ())
+  send_conf_auth_later = (fun tr1 tr2 sender receiver payload -> ())
 }
 
 #push-options "--ifuel 1 --fuel 0"
 let event_predicate_communication_layer 
   {|cinvs:crypto_invariants|}
-  (local_extension:comm_higher_layer_event_preds)
   (higher_layer_preds:comm_higher_layer_event_preds) : 
   event_predicate communication_event =
   fun tr prin e ->
     (match e with
     | CommConfSendMsg sender receiver payload -> (
       is_knowable_by (join (principal_label sender) (principal_label receiver)) tr payload /\
-      higher_layer_preds.send_conf tr sender receiver payload /\
-      local_extension.send_conf tr sender receiver payload
+      higher_layer_preds.send_conf tr sender receiver payload
     )
     | CommConfReceiveMsg receiver payload -> (
       exists sender.
@@ -282,38 +173,19 @@ let event_predicate_communication_layer
       event_triggered tr sender (CommConfAuthSendMsg sender receiver payload) \/
       is_corrupt tr (long_term_key_label sender)
     )
-    | CommClientSendRequest client server id payload -> (
-      is_knowable_by (comm_label client server) tr payload /\
-      higher_layer_preds.send_request tr client server payload
-    )
-    | CommServerReceiveRequest server id payload -> (
-      exists client. is_knowable_by (comm_label client server) tr payload /\
-      (event_triggered tr client (CommClientSendRequest client server id payload) \/
-        is_publishable tr payload)
-    )
-    | CommServerSendResponse server id payload -> (
-      (exists client. is_knowable_by (comm_label client server) tr payload) /\
-      higher_layer_preds.send_response tr server payload
-    )
-    | CommClientReceiveResponse client server id payload key -> (
-      event_triggered tr server (CommServerReceiveRequest server id payload) \/
-      is_corrupt tr (long_term_key_label server)
-    )
     )
 #pop-options
 
 val event_predicate_communication_layer_and_tag: 
   {|cinvs:crypto_invariants|} ->
   comm_higher_layer_event_preds ->
-  comm_higher_layer_event_preds ->
   (string & compiled_event_predicate)
-let event_predicate_communication_layer_and_tag #cinvs local_extension higher_layer_preds =
-  (event_communication_event.tag, compile_event_pred #communication_event (event_predicate_communication_layer #cinvs local_extension higher_layer_preds))
+let event_predicate_communication_layer_and_tag #cinvs higher_layer_preds =
+  (event_communication_event.tag, compile_event_pred (event_predicate_communication_layer #cinvs higher_layer_preds))
 
 val has_communication_layer_event_predicates:
   {|protocol_invariants|} ->
   comm_higher_layer_event_preds ->
-  comm_higher_layer_event_preds ->
   prop
-let has_communication_layer_event_predicates #invs local_extension higher_layer_preds =
-  has_event_pred (event_predicate_communication_layer local_extension higher_layer_preds)
+let has_communication_layer_event_predicates #invs higher_layer_preds =
+  has_event_pred (event_predicate_communication_layer #invs.crypto_invs higher_layer_preds)
