src/lib/communication/DY.Lib.Communication.RequestResponse.Invariants.fst
@@ -1,0 +1,223 @@
+module DY.Lib.Communication.RequestResponse.Invariants
+
+open Comparse
+open DY.Core
+open DY.Lib.Communication.Core.Extension
+open DY.Lib.Crypto.PkEncryption.Split
+open DY.Lib.Crypto.Signature.Split
+open DY.Lib.Crypto.AEAD.Split
+open DY.Lib.Event.Typed
+open DY.Lib.State.PrivateKeys
+open DY.Lib.State.Tagged
+open DY.Lib.State.Typed
+
+open DY.Lib.Communication.Core
+open DY.Lib.Communication.RequestResponse
+open DY.Lib.Communication.Core.Invariants
+
+#set-options "--fuel 0 --ifuel 0 --z3cliopt 'smt.qi.eager_threshold=100'"
+
+(*** AEAD Predicate ***)
+
+#push-options "--ifuel 1"
+val aead_crypto_predicate_communication_layer: {|cusages:crypto_usages|} -> aead_crypto_predicate
+let aead_crypto_predicate_communication_layer #cusages = {
+  pred = (fun tr key_usage nonce msg ad ->
+    (match parse response_message msg with
+    | None -> False
+    | Some {id; payload} -> (
+      match parse authenticated_data ad with
+      | None -> False
+      | Some {client; server} -> (
+          event_triggered tr server (CommServerSendResponse client server id payload) /\
+          (get_label tr id) `can_flow tr` (comm_label client server) /\
+          (get_label tr payload) `can_flow tr` (comm_label client server)
+      )
+    ))
+  );
+  pred_later = (fun tr1 tr2 key_usage nonce msg ad -> (
+    parse_wf_lemma response_message (bytes_well_formed tr1) msg;
+    parse_wf_lemma authenticated_data (bytes_well_formed tr1) ad;
+    ()
+  ))
+}
+#pop-options
+
+val aead_crypto_predicates_communication_layer_and_tag:
+  {|cusages:crypto_usages|} ->
+  (string & aead_crypto_predicate)
+let aead_crypto_predicates_communication_layer_and_tag #cusages =
+  (comm_layer_aead_tag, aead_crypto_predicate_communication_layer)
+
+val has_communication_layer_reqres_crypto_predicates:
+  {|cinvs:crypto_invariants|} ->
+  prop
+let has_communication_layer_reqres_crypto_predicates #cinvs =
+  // Fix for the get_label function in the model code
+  cinvs.usages == default_crypto_usages /\
+  has_pkenc_predicate pkenc_crypto_predicates_communication_layer_and_tag /\
+  has_sign_predicate sign_crypto_predicates_communication_layer_and_tag /\
+  has_aead_predicate aead_crypto_predicates_communication_layer_and_tag
+
+
+(*** State Predicates ***)
+
+#push-options "--ifuel 2 --z3rlimit 25"
+let state_predicates_communication_layer {|crypto_invariants|}: local_state_predicate communication_states = {
+  pred = (fun tr prin sess_id st -> 
+    match st with
+    | ClientSendRequest {id; server; payload; key} -> (
+      let client = prin in
+      is_secret (comm_label client server) tr id /\
+      is_knowable_by (comm_label client server) tr payload /\
+      is_secret (comm_label client server) tr key /\
+      key `has_usage tr` (AeadKey comm_layer_aead_tag empty)
+    )
+    | ServerReceiveRequest {id; client; payload; key} -> (
+      let server = prin in
+      ( //exists client.
+        is_knowable_by (comm_label client server) tr key /\
+        is_knowable_by (get_label tr key) tr payload
+      ) /\
+      (
+        key `has_usage tr` (AeadKey comm_layer_aead_tag empty) \/
+        is_publishable tr key
+      ) /\
+      is_knowable_by (get_label tr key) tr id
+    )
+    | ClientReceiveResponse {id; server; payload; key} -> (
+      let client = prin in
+      is_secret (comm_label client server) tr id /\
+      is_knowable_by (comm_label client server) tr payload /\
+      is_secret (comm_label client server) tr key
+    )
+  );
+  pred_later = (fun tr1 tr2 prin sess_id state -> ());
+  pred_knowable = (fun tr prin sess_id state -> ());
+}
+#pop-options
+
+val state_predicates_communication_layer_and_tag: 
+  {|crypto_invariants|} ->
+  dtuple2 string local_bytes_state_predicate
+let state_predicates_communication_layer_and_tag #cinvs =
+  (|local_state_communication_layer_session.tag, local_state_predicate_to_local_bytes_state_predicate (state_predicates_communication_layer #cinvs)|)
+
+val has_communication_layer_state_predicates:
+  {|protocol_invariants|} ->
+  prop
+let has_communication_layer_state_predicates #invs =
+  has_local_state_predicate state_predicates_communication_layer
+
+
+(*** Event Predicates ***)
+
+noeq
+type comm_reqres_higher_layer_event_preds = {
+  send_request: tr:trace -> client:principal -> server:principal -> payload:bytes -> key_label:label -> prop;
+  send_request_later:
+    tr1:trace -> tr2:trace ->
+    client:principal -> server:principal -> payload:bytes -> key_label:label ->
+    Lemma
+    (requires
+      send_request tr1 client server payload key_label /\
+      bytes_well_formed tr1 payload /\
+      tr1 <$ tr2
+    )
+    (ensures
+      send_request tr2 client server payload key_label
+    )
+  ;
+  send_response: tr:trace -> server:principal -> payload:bytes -> prop;
+  send_response_later:
+    tr1:trace -> tr2:trace ->
+    server:principal -> payload:bytes ->
+    Lemma
+    (requires
+      send_response tr1 server payload /\
+      bytes_well_formed tr1 payload /\
+      tr1 <$ tr2
+    )
+    (ensures
+      send_response tr2 server payload
+    )
+}
+
+val default_comm_reqres_higher_layer_event_preds: comm_reqres_higher_layer_event_preds
+let default_comm_reqres_higher_layer_event_preds = {
+  send_request = (fun tr client server payload key_label -> True);
+  send_request_later = (fun tr1 tr2 client server payload key_label -> ());
+  send_response = (fun tr server payload -> True);
+  send_response_later = (fun tr1 tr2 server payload -> ())
+}
+
+#push-options "--ifuel 1 --fuel 0"
+let event_predicate_communication_layer_reqres
+  {|cinvs:crypto_invariants|}
+  (higher_layer_resreq_preds:comm_reqres_higher_layer_event_preds) : 
+  event_predicate communication_reqres_event =
+  fun tr prin e ->
+    (match e with
+    | CommClientSendRequest client server id payload key -> (
+      is_knowable_by (get_label tr key) tr payload /\
+      is_secret (comm_label client server) tr key /\
+      is_secret (get_label tr key) tr id /\
+      key `has_usage tr` (AeadKey comm_layer_aead_tag empty) /\
+      higher_layer_resreq_preds.send_request tr client server payload (get_label tr key)
+    )
+    | CommServerReceiveRequest client server id payload key -> (
+      is_knowable_by (comm_label client server) tr payload /\
+      (event_triggered tr client (CommClientSendRequest client server id payload key) \/
+        is_publishable tr payload)
+    )
+    | CommServerSendResponse client server id payload -> (
+      higher_layer_resreq_preds.send_response tr server payload
+    )
+    | CommClientReceiveResponse client server id payload key -> (
+      event_triggered tr server (CommServerReceiveRequest client server id payload key) \/
+      is_corrupt tr (long_term_key_label server)
+    )
+    )
+#pop-options
+
+// Additional event preconditions for the events from the core communication layer
+#push-options "--fuel 0 --ifuel 1"
+val request_response_event_preconditions: {|cinvs:crypto_invariants|} -> comm_higher_layer_event_preds
+let request_response_event_preconditions #cinvs = {
+  default_comm_higher_layer_event_preds with
+  send_conf = (fun tr client server req_payload -> (
+      match decode_request_message req_payload with
+      | None -> False
+      | Some {id; client=client'; payload; key} -> (
+        client == client' /\
+        //is_knowable_by (get_label tr key) tr id /\
+        event_triggered tr client (CommClientSendRequest client server id payload key)
+      )
+    )
+  );
+  send_conf_later = (fun tr1 tr2 client server req_payload -> (
+      parse_wf_lemma request_message (bytes_well_formed tr1) req_payload;
+      ()
+    )
+  )
+}
+#pop-options
+
+val event_predicate_communication_layer_reqres_and_tag: 
+  {|cinvs:crypto_invariants|} ->
+  comm_reqres_higher_layer_event_preds ->
+  list (string & compiled_event_predicate)
+let event_predicate_communication_layer_reqres_and_tag #cinvs higher_layer_resreq_preds =
+  [
+    event_predicate_communication_layer_and_tag request_response_event_preconditions;
+    event_communication_reqres_event.tag, compile_event_pred (event_predicate_communication_layer_reqres #cinvs higher_layer_resreq_preds)
+  ]
+
+val has_communication_layer_reqres_event_predicates:
+  {|protocol_invariants|} ->
+  comm_higher_layer_event_preds ->
+  comm_reqres_higher_layer_event_preds ->
+  prop
+let has_communication_layer_reqres_event_predicates #invs higher_layer_preds higher_layer_resreq_preds =
+  has_event_pred (event_predicate_communication_layer #invs.crypto_invs higher_layer_preds) /\
+  has_event_pred (event_predicate_communication_layer_reqres #invs.crypto_invs higher_layer_resreq_preds)
